Prove lemmas/statelemmas with tainted semantics

src/arch/x64/X64.Vale.Lemmas_i.fst
@@ -1,8 +1,12 @@
 module X64.Vale.Lemmas_i
 open X64.Machine_s
 open X64.Vale.State_i
+open X64.Vale.StateLemmas_i
 open FStar.UInt
+open FStar.FunctionalExtensionality
+open FStar.Tactics
 module S = X64.Semantics_s
+module TS = X64.Taint_Semantics_s
 
 #reset-options "--initial_fuel 2 --max_fuel 2 --z3rlimit 20"
 
@@ -21,45 +25,53 @@ let rec increase_fuel (c:code) (s0:state) (f0:fuel) (sN:state) (fN:fuel) =
   | Ins ins -> ()
   | Block l -> increase_fuels l s0 f0 sN fN
   | IfElse b t f ->
-      let s0 = ensure_valid_ocmp b s0 in
-      if eval_ocmp s0 b then increase_fuel t s0 f0 sN fN else increase_fuel f s0 f0 sN fN
+      let s1 = ensure_valid_ocmp b s0 in
+      let b0 = eval_ocmp s1 b in
+      let s2 = {s1 with trace = BranchPredicate(b0)::s1.trace} in
+      assert (feq ((state_to_S ({s1 with trace = BranchPredicate(b0)::s1.trace})).TS.state.S.regs)
+	({(state_to_S s1) with TS.trace = BranchPredicate(b0)::(state_to_S s1).TS.trace}).TS.state.S.regs);
+      if b0 then increase_fuel t s2 f0 sN fN else increase_fuel f s2 f0 sN fN
   | While b c ->
       let s0 = ensure_valid_ocmp b s0 in
-      if not (eval_ocmp s0 b) then ()
+      let b0 = eval_ocmp s0 b in
+      if not b0 then ()
       else
       (
-        match S.eval_code c (f0 - 1) (state_to_S s0) with
+	let s1 = {s0 with trace = BranchPredicate(true)::s0.trace} in
+	assert (feq ((state_to_S ({s0 with trace = BranchPredicate(true)::s0.trace})).TS.state.S.regs)
+	({(state_to_S s0) with TS.trace = BranchPredicate(b0)::(state_to_S s0).TS.trace}).TS.state.S.regs);
+        match TS.taint_eval_code c (f0 - 1) (state_to_S s1) with
         | None -> ()
-        | Some s1 ->
-            let s1 = state_of_S s1 in
-            increase_fuel c s0 (f0 - 1) s1 (fN - 1);
-            if s1.ok then increase_fuel (While b c) s1 (f0 - 1) sN (fN - 1)
+        | Some s2 ->
+            let s2 = state_of_S s2 in
+            increase_fuel c s1 (f0 - 1) s2 (fN - 1);
+            if s2.ok then increase_fuel (While b c) s2 (f0 - 1) sN (fN - 1)
             else ()
-      )
+      ) 
 and increase_fuels (c:codes) (s0:state) (f0:fuel) (sN:state) (fN:fuel) =
   match c with
   | [] -> ()
   | h::t ->
     (
-      let Some s1 = S.eval_code h f0 (state_to_S s0) in
+      let Some s1 = TS.taint_eval_code h f0 (state_to_S s0) in
       let s1 = state_of_S s1 in
       increase_fuel h s0 f0 s1 fN;
       increase_fuels t s1 f0 sN fN
     )
 
-let lemma_cmp_eq s o1 o2 = ()
-let lemma_cmp_ne s o1 o2 = ()
-let lemma_cmp_le s o1 o2 = ()
-let lemma_cmp_ge s o1 o2 = ()
-let lemma_cmp_lt s o1 o2 = ()
-let lemma_cmp_gt s o1 o2 = ()
+let lemma_cmp_eq s o1 o2 t = ()
+let lemma_cmp_ne s o1 o2 t = ()
+let lemma_cmp_le s o1 o2 t = ()
+let lemma_cmp_ge s o1 o2 t = ()
+let lemma_cmp_lt s o1 o2 t = ()
+let lemma_cmp_gt s o1 o2 t = ()
 
-let lemma_valid_cmp_eq s o1 o2 = ()
-let lemma_valid_cmp_ne s o1 o2 = ()
-let lemma_valid_cmp_le s o1 o2 = ()
-let lemma_valid_cmp_ge s o1 o2 = ()
-let lemma_valid_cmp_lt s o1 o2 = ()
-let lemma_valid_cmp_gt s o1 o2 = ()
+let lemma_valid_cmp_eq s o1 o2 t = ()
+let lemma_valid_cmp_ne s o1 o2 t = ()
+let lemma_valid_cmp_le s o1 o2 t = ()
+let lemma_valid_cmp_ge s o1 o2 t = ()
+let lemma_valid_cmp_lt s o1 o2 t = ()
+let lemma_valid_cmp_gt s o1 o2 t = ()
 
 let lemma_merge_total (b0:codes) (s0:state) (f0:fuel) (sM:state) (fM:fuel) (sN:state) =
   let f = if f0 > fM then f0 else fM in
@@ -74,15 +86,19 @@ let lemma_ifElse_total (ifb:ocmp) (ct:code) (cf:code) (s0:state) =
   (eval_ocmp s0 ifb, s0, s0, 0)
 
 let lemma_ifElseTrue_total (ifb:ocmp) (ct:code) (cf:code) (s0:state) (f0:fuel) (sM:state) =
+  assert (feq ((state_to_S ({s0 with trace = BranchPredicate(true)::s0.trace})).TS.state.S.regs)
+    ({(state_to_S s0) with TS.trace = BranchPredicate(true)::(state_to_S s0).TS.trace}).TS.state.S.regs);
   ()
 
 let lemma_ifElseFalse_total (ifb:ocmp) (ct:code) (cf:code) (s0:state) (f0:fuel) (sM:state) =
+  assert (feq ((state_to_S ({s0 with trace = BranchPredicate(false)::s0.trace})).TS.state.S.regs)
+    ({(state_to_S s0) with TS.trace = BranchPredicate(false)::(state_to_S s0).TS.trace}).TS.state.S.regs);
   ()
 
 let eval_while_inv_temp (c:code) (s0:state) (fW:fuel) (sW:state) : Type0 =
-  forall (f:nat).{:pattern S.eval_code c f (state_to_S sW)}
-    Some? (S.eval_code c f (state_to_S sW)) ==>
-    S.eval_code c (f + fW) (state_to_S s0) == S.eval_code c f (state_to_S sW)
+  forall (f:nat).{:pattern TS.taint_eval_code c f (state_to_S sW)}
+    Some? (TS.taint_eval_code c f (state_to_S sW)) ==>
+    TS.taint_eval_code c (f + fW) (state_to_S s0) == TS.taint_eval_code c f (state_to_S sW)
 
 let eval_while_inv (c:code) (s0:state) (fW:fuel) (sW:state) : Type0 =
   eval_while_inv_temp c s0 fW sW
@@ -95,25 +111,28 @@ let lemma_whileTrue_total (b:ocmp) (c:code) (s0:state) (sW:state) (fW:fuel) =
 
 let lemma_whileFalse_total (b:ocmp) (c:code) (s0:state) (sW:state) (fW:fuel) =
   let f1 = fW + 1 in
-  assert (S.eval_code (While b c) f1 (state_to_S s0) == S.eval_code (While b c) 1 (state_to_S sW));
-  assert (eval_code (While b c) s0 f1 sW);
-  (sW, f1)
+  assert (TS.taint_eval_code (While b c) f1 (state_to_S s0) == TS.taint_eval_code (While b c) 1 (state_to_S sW));
+  assert (feq ((state_to_S ({sW with trace = BranchPredicate(false)::sW.trace})).TS.state.S.regs)
+    ({(state_to_S sW) with TS.trace = BranchPredicate(false)::(state_to_S sW).TS.trace}).TS.state.S.regs);
+  assert (eval_code (While b c) s0 f1 ({sW with trace = BranchPredicate(false)::sW.trace}));
+  ({sW with trace = BranchPredicate(false)::sW.trace}, f1)
   
 #reset-options "--initial_fuel 2 --max_fuel 2 --z3rlimit 30"
 let lemma_whileMerge_total (c:code) (s0:state) (f0:fuel) (sM:state) (fM:fuel) (sN:state) =
   let fN:nat = f0 + fM + 1 in
   let fForall (f:nat) : Lemma
-    (requires Some? (S.eval_code c f (state_to_S sN)))
-    (ensures S.eval_code c (f + fN) (state_to_S s0) == S.eval_code c f (state_to_S sN)) =
-    let Some sZ = S.eval_code c f (state_to_S sN) in
+    (requires Some? (TS.taint_eval_code c f (state_to_S sN)))
+    (ensures TS.taint_eval_code c (f + fN) (state_to_S s0) == TS.taint_eval_code c f (state_to_S sN)) =
+    let Some sZ = TS.taint_eval_code c f (state_to_S sN) in
     let fZ = if f > fM then f else fM in
-    increase_fuel (While?.whileBody c) sM fM sN fZ;
+    increase_fuel (While?.whileBody c) ({sM with trace = BranchPredicate(true)::sM.trace}) fM sN fZ;
     increase_fuel c sN f (state_of_S sZ) fZ;
-    assert (S.eval_code c (fZ + 1) (state_to_S sM) == Some sZ);
-    assert (S.eval_code c (fZ + 1) (state_to_S sM) == S.eval_code c (fZ + 1 + f0) (state_to_S s0));
-    assert (S.eval_code c (fZ + 1 + f0) (state_to_S s0) == Some sZ);
+    assert (feq ((state_to_S ({sM with trace = BranchPredicate(true)::sM.trace})).TS.state.S.regs) ({(state_to_S sM) with TS.trace = BranchPredicate(true)::(state_to_S sM).TS.trace}).TS.state.S.regs);
+    assert (TS.taint_eval_code c (fZ + 1) (state_to_S sM) == Some sZ);
+    assert (TS.taint_eval_code c (fZ + 1) (state_to_S sM) == TS.taint_eval_code c (fZ + 1 + f0) (state_to_S s0));
+    assert (TS.taint_eval_code c (fZ + 1 + f0) (state_to_S s0) == Some sZ);
     increase_fuel c s0 (fZ + 1 + f0) (state_of_S sZ) (f + fN);
-    assert (S.eval_code c (f + fN) (state_to_S s0) == Some sZ);
+    assert (TS.taint_eval_code c (f + fN) (state_to_S s0) == Some sZ);
     ()
     in
   Classical.ghost_lemma fForall;
