src/arch/x64/X64.Vale.StateLemmas_i.fst
@@ -3,31 +3,19 @@ open X64.Machine_s
 open X64.Vale.State_i
 open FStar.UInt
 module S = X64.Semantics_s
+module TS = X64.Taint_Semantics_s
 module M = TransparentMap
 
 #reset-options "--initial_fuel 2 --max_fuel 2"
-
-let state_to_S (s:state) : S.state = {
-  S.ok = s.ok;
-  S.regs = (fun r -> s.regs r);
-  S.flags = int_to_nat64 s.flags;
-  S.mem = s.mem;
-}
-
-let state_of_S (s:S.state) : state =
-  let { S.ok = ok; S.regs = regs; S.flags = flags; S.mem = mem } = s in {
-    ok = ok;
-    regs = (fun r -> regs r);
-    flags = flags;
-    mem = mem;
-  }
 
 let lemma_to_ok s = ()
 let lemma_to_flags s = ()
 let lemma_to_mem s = ()
 let lemma_to_reg s r = ()
+let lemma_to_trace s = ()
+let lemma_to_memTaint s = ()
 let lemma_to_eval_operand s o = ()
-let lemma_to_valid_operand s o = ()
+let lemma_to_valid_operand s o t = ()
 
 let lemma_of_to s =
   assert (state_eq s (state_of_S (state_to_S s)));
@@ -36,7 +24,15 @@ let lemma_of_to s =
 let lemma_to_of s =
   let s' = state_of_S s in
   let s'' = state_to_S s' in
-  let { S.ok = ok; S.regs = regs; S.flags = flags; S.mem = mem } = s in
-  let { S.ok = ok''; S.regs = regs''; S.flags = flags''; S.mem = mem'' } = s'' in
+  let { S.ok = ok; S.regs = regs; S.flags = flags; S.mem = mem } = s.TS.state in
+  let { S.ok = ok''; S.regs = regs''; S.flags = flags''; S.mem = mem'' } = s''.TS.state in
   assert (feq regs regs'');
+  ()
+
+let lemma_regs_inv s1 s2 =
+  let s1' = state_to_S s1 in
+  let s2' = state_to_S s2 in
+  let regs1 = s1'.TS.state.S.regs in
+  let regs2 = s2'.TS.state.S.regs in
+  assert (s1.regs == s2.regs ==> feq regs1 regs2);
   ()
