src/arch/x64/X64.Vale.StateLemmas_i.fsti
@@ -4,45 +4,77 @@ open X64.Vale.State_i
 open FStar.UInt
 open FStar.FunctionalExtensionality
 module S = X64.Semantics_s
+module TS = X64.Taint_Semantics_s
 module M = TransparentMap
 
 unfold let ok' = S.Mkstate?.ok
 unfold let regs' = S.Mkstate?.regs
 unfold let flags' = S.Mkstate?.flags
 unfold let mem' = S.Mkstate?.mem
+unfold let trace' = TS.MktraceState?.trace
+unfold let memTaint' = TS.MktraceState?.memTaint
 
-val state_to_S : s:state -> S.state
-val state_of_S : s:S.state -> state
+let state_to_S (s:state) : TS.traceState = {
+  TS.state = {
+    S.ok = s.ok;
+    S.regs = (fun r -> s.regs r);
+    S.flags = int_to_nat64 s.flags;
+    S.mem = s.mem;
+  };
+  TS.trace = s.trace;
+  TS.memTaint = s.memTaint;
+}
+
+let state_of_S (s:TS.traceState) : state =
+  let { S.ok = ok; S.regs = regs; S.flags = flags; S.mem = mem } = s.TS.state in {
+    ok = ok;
+    regs = (fun r -> regs r);
+    flags = flags;
+    mem = mem;
+    trace = s.TS.trace;
+    memTaint = s.TS.memTaint
+  }
 
 val lemma_to_ok : s:state -> Lemma
-  (ensures s.ok == ok' (state_to_S s))
+  (ensures s.ok == ok' ((state_to_S s).TS.state))
   [SMTPat s.ok]
 
 val lemma_to_flags : s:state -> Lemma
-  (ensures s.flags == flags' (state_to_S s))
+  (ensures s.flags == flags' ((state_to_S s).TS.state))
   [SMTPat s.flags]
 
 val lemma_to_mem : s:state -> Lemma
-  (ensures s.mem == mem' (state_to_S s))
+  (ensures s.mem == mem' ((state_to_S s).TS.state))
   [SMTPat s.mem]
   
 val lemma_to_reg : s:state -> r:reg -> Lemma
-  (ensures s.regs r == regs' (state_to_S s) r)
+  (ensures s.regs r == regs' ((state_to_S s).TS.state) r)
   [SMTPat (s.regs r)]
 
+val lemma_to_trace : s:state -> Lemma
+  (ensures s.trace == trace' (state_to_S s))
+  [SMTPat s.trace]
+
+val lemma_to_memTaint : s:state -> Lemma
+  (ensures s.memTaint == memTaint' (state_to_S s))
+  [SMTPat s.memTaint]
+
 val lemma_to_eval_operand : s:state -> o:operand -> Lemma
-  (ensures eval_operand o s == S.eval_operand o (state_to_S s))
+  (ensures eval_operand o s == S.eval_operand o ((state_to_S s).TS.state))
   [SMTPat (eval_operand o s)]
 
-val lemma_to_valid_operand : s:state -> o:operand -> Lemma
-  (ensures valid_operand o s ==> S.valid_operand o (state_to_S s))
-  [SMTPat (valid_operand o s)]
+val lemma_to_valid_operand : s:state -> o:operand -> t:taint -> Lemma
+  (ensures valid_operand o s t ==> S.valid_operand o ((state_to_S s).TS.state) /\ TS.taint_match o t (state_to_S s).TS.memTaint (state_to_S s).TS.state)
+  [SMTPat (valid_operand o s t)]
 
 val lemma_of_to : s:state -> Lemma
   (ensures s == state_of_S (state_to_S s))
   [SMTPat (state_of_S (state_to_S s))]
 
-val lemma_to_of : s:S.state -> Lemma
+val lemma_to_of : s:TS.traceState -> Lemma
   (ensures s == state_to_S (state_of_S s))
   [SMTPat (state_to_S (state_of_S s))]
 
+val lemma_regs_inv : s1:state -> s2:state -> Lemma
+  (ensures s1.regs == s2.regs ==> regs' ((state_to_S s1).TS.state) == regs' ((state_to_S s2).TS.state))
+  [SMTPat ((state_to_S s1).TS.state.S.regs == (state_to_S s2).TS.state.S.regs)]
